<?xml version='1.0'?>

<!DOCTYPE rdf:RDF [
    <!ENTITY jena    'http://jena.hpl.hp.com/schemas/'>

    <!ENTITY rdf     'http://www.w3.org/1999/02/22-rdf-syntax-ns#'>
    <!ENTITY rdfs    'http://www.w3.org/2000/01/rdf-schema#'>
    <!ENTITY owl     'http://www.w3.org/2002/07/owl#'>
    <!ENTITY xsd     'http://www.w3.org/2001/XMLSchema#'>
    <!ENTITY dc      'http://purl.org/dc/elements/1.1/'>
    <!ENTITY base    '&jena;2003/03/ont-manager'>
    <!ENTITY ont     '&base;#'>
]>

<rdf:RDF
  xmlns:rdf ="&rdf;"
  xmlns:rdfs="&rdfs;"
  xmlns:dc  ="&dc;"
  xmlns:owl ="&owl;"
  xmlns     ="&ont;"
  xml:base  ="&base;"
>

<owl:Ontology rdf:about="">
  <rdfs:comment>
	A simple schema (vocabulary) for the properties used to store metadata for the Jena ontology document manager.
  </rdfs:comment>

  <dc:creator>
    Ian Dickinson, mailto:ian_dickinson@users.sourceforge.net
  </dc:creator>

  <owl:versionInfo>
	CVS:    $Id: ont-manager.rdf,v 1.5 2009-10-06 13:04:42 ian_dickinson Exp $
  </owl:versionInfo>
</owl:Ontology>

<rdfs:Class rdf:ID="OntologySpec">
	<rdfs:label>Ontology document specification</rdfs:label>
	<rdfs:comment>A class of node that specifies document metadata for the DocumentManager</rdfs:comment>
</rdfs:Class>

<rdf:Property rdf:ID="publicURI">
	<rdfs:label>Public URI</rdfs:label>
	<rdfs:comment>The public URI that is used to refer to the ontology document</rdfs:comment>
	<rdfs:domain rdf:resource="#OntologySpec" />
</rdf:Property>

<rdf:Property rdf:ID="altURL">
	<rdfs:label>Alternative URL</rdfs:label>
	<rdfs:comment>The resolvable URL that an alternative copy of the ontology document may be fetched from</rdfs:comment>
	<rdfs:domain rdf:resource="#OntologySpec" />
</rdf:Property>

<rdf:Property rdf:ID="prefix">
	<rdfs:label>Prefix</rdfs:label>
	<rdfs:comment>The prefix string that is used when writing qnames in the ontology's namespace</rdfs:comment>
	<rdfs:domain rdf:resource="#OntologySpec" />
	<rdfs:range rdf:resource="&xsd;string" />
</rdf:Property>

<rdf:Property rdf:ID="language">
	<rdfs:label>Ontology language</rdfs:label>
	<rdfs:comment>The representation language used by the ontology document</rdfs:comment>
	<rdfs:domain rdf:resource="#OntologySpec" />
</rdf:Property>



<rdfs:Class rdf:ID="DocumentManagerPolicy">
	<rdfs:label>Ontology document manager policy</rdfs:label>
	<rdfs:comment>A node that specifies behavioural options for the document manager</rdfs:comment>
</rdfs:Class>

<rdf:Property rdf:ID="cacheModels">
	<rdfs:label>cache models</rdfs:label>
	<rdfs:comment>If true, this property denotes that loaded models should be cached for re-use</rdfs:comment>
	<rdfs:domain rdf:resource="#DocumentManagerPolicy" />
	<rdfs:range rdf:resource="&xsd;boolean" />
</rdf:Property>

<rdf:Property rdf:ID="processImports">
	<rdfs:label>process imports</rdfs:label>
	<rdfs:comment>If true, this property denotes that the document manager should process the imports closure of documents</rdfs:comment>
	<rdfs:domain rdf:resource="#DocumentManagerPolicy" />
	<rdfs:range rdf:resource="&xsd;boolean" />
</rdf:Property>

<rdf:Property rdf:ID="ignoreImport">
	<rdfs:label>Ignore specified import</rdfs:label>
	<rdfs:comment>Specifies URL that will never be loaded as the result of processing an imports statement</rdfs:comment>
	<rdfs:domain rdf:resource="#DocumentManagerPolicy" />
</rdf:Property>

<rdf:Property rdf:ID="useDeclaredNsPrefixes">
	<rdfs:label>Use declared NS prefixes</rdfs:label>
	<rdfs:comment>Boolean flag for whether new ontology models will include the pre-declared namespace prefixes</rdfs:comment>
	<rdfs:domain rdf:resource="#DocumentManagerPolicy" />
</rdf:Property>


</rdf:RDF>
